push work so far

src/Std/Data/DHashMap/Internal/Defs.lean
@@ -480,6 +480,10 @@ def interSmaller [BEq α] [Hashable α] (m₁ : Raw₀ α β) (m₂ : Raw α β)
 def inter [BEq α] [Hashable α] (m₁ m₂ : Raw₀ α β) : Raw₀ α β :=
   if m₁.1.size ≤ m₂.1.size then m₁.filter fun k _ => m₂.contains k else interSmaller m₁ m₂
 
+/-- Internal implementation detail of the hash map -/
+def checkBEq [BEq α] [LawfulBEq α] [Hashable α] [∀ k, BEq (β k)] (m₁ m₂ : Raw₀ α β) : Bool :=
+  if m₁.1.size ≠ m₂.1.size then false else m₁.1.all (fun k v => m₂.get? k == some v)
+
 section
 
 variable {β : Type v}
